progs/conclib.v
@@ -506,6 +506,22 @@ Proof.
     + f_equal; omega.
 Qed.
 
+Lemma upd_complete_gen : forall {A} (l : list A) x n y, Zlength l < n ->
+  upd_Znth (Zlength l) (l ++ repeat y (Z.to_nat (n - Zlength l))) x =
+  (l ++ [x]) ++ repeat y (Z.to_nat (n - Zlength (l ++ [x]))).
+Proof.
+  intros.
+  rewrite upd_Znth_app2, Zminus_diag.
+  destruct (Z.to_nat (n - Zlength l)) eqn: Hn.
+  - apply Z2Nat.inj with (m := 0) in Hn; omega.
+  - simpl; rewrite upd_Znth0, Zlength_cons, sublist_1_cons.
+    unfold Z.succ; rewrite Z.add_simpl_r, sublist_same; auto.
+    rewrite <- app_assoc, Zlength_app, Zlength_cons, Zlength_nil; simpl.
+    rewrite Z.sub_add_distr, Z2Nat.inj_sub, Hn by computable; simpl.
+    rewrite Nat.sub_0_r; auto.
+  - pose proof (Zlength_nonneg (repeat y (Z.to_nat (n - Zlength l)))); omega.
+Qed.
+
 Lemma upd_complete' : forall l x n, (length l < n)%nat ->
   upd_Znth (Zlength l) (map Vint (map Int.repr l) ++ repeat Vundef (n - length l)) (Vint (Int.repr x)) =
   map Vint (map Int.repr (l ++ [x])) ++ repeat Vundef (n - length (l ++ [x])).
